Cleaned up a bit the closure conversion files. Moved several lemmas to the appropriate files. Added new file (functions.v) with useful definitions and lemmas about functions (extensional equality, image, codomain, injectiveity, etc…) that are useful for name substitutions.

theories/L6_PCPS/alpha_conv.v
@@ -1,5 +1,5 @@
 Require Import cps ctx cps_util set_util identifiers Ensembles_util List_util
-        eval logical_relations.
+        eval logical_relations functions.
 Require Import Coq.ZArith.Znumtheory Coq.Relations.Relations Coq.Arith.Wf_nat.
 Require Import Coq.Lists.List Coq.MSets.MSets Coq.MSets.MSetRBT Coq.Numbers.BinNums
         Coq.NArith.BinNat Coq.PArith.BinPos Coq.Sets.Ensembles Omega.
@@ -7,14 +7,8 @@ Require Import Coq.Lists.List Coq.MSets.MSets Coq.MSets.MSetRBT Coq.Numbers.BinN
 Import ListNotations.
 
 Open Scope ctx_scope.
+Open Scope fun_scope.
 
-Definition extend (f: var -> var) (x x' : var) : (var -> var) :=
-  fun z => if Coqlib.peq z x then x' else f z.
-
-Notation " f '{' x '~>' y '}' " := (extend f x y) (at level 10, no associativity)
-                                   : alpha_scope.
-
-Open Scope alpha_scope.
 
 Fixpoint extend_lst (f: var -> var) (xs xs' : list var) : (var -> var) :=
   match xs with
@@ -44,19 +38,6 @@ Fixpoint extend_fundefs (f: var -> var) (B B' : fundefs) : (var -> var) :=
 (* Notation " f '<{' B '~>' B' '}>' " := (extend_fundefs f B B') (at level 10, no associativity) *)
 (*                                        : alpha_scope. *)
 
-Definition codomain {A B} (f : A -> B) : Ensemble B := 
-  fun y => exists x, f x = y.
-
-Definition image {A B} (f : A -> B) (S : Ensemble A) :=
-  fun y => exists x, In _ S x /\ f x = y.
-
-(** A function is injective in a subdomain *)
-Definition injectiveP {A B} (f : A -> B) P :=
-  forall x x', In _ P x -> In _ P x' -> f x = f x' -> x = x'.
-
-Definition injective {A B} (f : A -> B) :=
-  forall x x', f x = f x' -> x = x'.
-
 Inductive construct_lst_injection : (var -> var) -> list var -> list var -> (var -> var) -> Prop :=
 | Inj_nil :
     forall f, construct_lst_injection f [] [] f
@@ -75,6 +56,7 @@ Inductive construct_fundefs_injection : (var -> var) -> fundefs -> fundefs -> (v
       injective (f' {g1 ~> g2}) ->
       construct_fundefs_injection f (Fcons g1 t1 xs1 e1 B1) (Fcons g2 t2 xs2 e2 B2) (f' {g1 ~> g2}).
 
+(** α-equivalent terms *)
 Inductive Alpha_conv : exp -> exp -> (var -> var) -> Prop :=
 | Alpha_Econstr :
     forall x x' tau t ys ys' e e' f,
@@ -122,66 +104,6 @@ with Alpha_conv_fundefs : fundefs -> fundefs -> (var -> var) -> Prop :=
       Alpha_conv e e' f' ->
       Alpha_conv_fundefs (Fcons g tau xs e B) (Fcons g' tau xs' e' B') f.
 
-Lemma extend_injective (f : var -> var) x y :
-  injective f ->
-  ~ In _ (codomain f) y ->
-  injective (f{x ~> y}).
-Proof.
-  intros Hinj Hin x1 x2 Heq.
-  unfold extend in *.
-  edestruct (Coqlib.peq x1 x).
-  - rewrite <- e in Heq.
-    edestruct (Coqlib.peq x2 x1); [ now eauto |].
-    exfalso. eapply Hin. eexists; eauto.
-  - edestruct (Coqlib.peq x2 x).
-    + exfalso. eapply Hin. eexists; eauto.
-    + eauto.
-Qed.
-
-Definition f_eq  {A B} (f f' : A -> B) : Prop :=
-    forall x, f x = f' x.
-
-Lemma f_eq_extend (f f' : var -> var) x y :
-  f_eq f f' ->
-  f_eq (f{x ~> y}) (f'{x ~> y}).
-Proof. 
-  intros Heq. 
-  unfold extend. intros z. 
-  destruct (Coqlib.peq z x); eauto.
-Qed.
-
-Lemma f_eq_extend_same (f : var -> var) x y :
-  f x = y ->
-  f_eq (f{x ~> y}) f.
-Proof. 
-  intros Heq x'.
-    unfold extend. destruct (Coqlib.peq x' x); eauto.
-    congruence. 
-Qed.    
-
-Lemma extend_same f x y :
-  f x = x ->
-  f {y ~> y} x = x. 
-Proof.
-  unfold extend. destruct (Coqlib.peq x y); eauto.
-Qed.
-
-Instance extend_Proper : Proper (f_eq ==> Logic.eq ==> Logic.eq ==> f_eq) extend.
-Proof. 
-  intros f1 f2 Hfeq x1 x2 Heq1 x3 x4 Hfeq2; subst.
-  intros x. unfold extend. destruct (Coqlib.peq x x2); eauto.
-Qed.
-
-Instance injective_proper {A B} : Proper (f_eq ==> iff) (@injective A B).
-Proof. 
-  intros f f' Heq. split; intros Hinj x y Heq'; eapply Hinj; congruence.
-Qed.
-
-Instance equivalence_f_eq {A B} : Equivalence (@f_eq A B). 
-Proof. 
-  constructor; congruence. 
-Qed.      
-
 Lemma construct_fundefs_injection_f_eq f f' B B' g :
   construct_fundefs_injection f B B' f' ->
   f_eq f g ->
@@ -219,18 +141,19 @@ Proof.
   eapply exp_def_mutual_ind; intros; split; intros H'; subst.
   - inv H'; constructor; eauto.
     + eapply Forall2_monotonic; [| eassumption ].
-      intros x1 x2 Heq. rewrite <- H2. eassumption. 
+      intros x1 x2 Heq. rewrite <- H2. eassumption.
     + rewrite f_eq_extend. eassumption. symmetry. eassumption.
     + eapply H; eauto. symmetry.
       eapply f_eq_extend. eassumption. 
   - inv H'; constructor; eauto.
     + eapply Forall2_monotonic; [| eassumption ].
-      intros x1 x2 Heq. rewrite H2. eassumption. 
+      intros x1 x2 Heq. rewrite H2. eassumption.
     + rewrite f_eq_extend. eassumption. eassumption.
     + eapply H; eauto.
       eapply f_eq_extend. eassumption. 
-  - inv H'. inv H2. constructor; eauto.
-  - inv H'. inv H2. constructor; eauto.
+  - inv H'. inv H2. constructor. constructor.
+    rewrite H1. reflexivity.
+  - inv H'. inv H2. constructor;  eauto.
   - inv H'; constructor; eauto. inv H4. destruct y as [c' e'].
     inv H5. simpl in H1; subst. constructor.
     split; eauto. eapply H; eauto. symmetry; eassumption.      
@@ -300,8 +223,6 @@ Proof.
   now apply Alpha_conv_proper_mut.
 Qed.
 
-
-
 (** Pair of contexts that preserves α-equivalence *)
 Definition Alpha_conv_ctx C C' f :=
   forall e e',
@@ -362,8 +283,9 @@ Proof.
     rewrite M.gss in Hget. inv Hget. eexists. rewrite M.gss; eauto.
   - intros z' Hget. rewrite M.gso in Hget; eauto.
     destruct (Coqlib.peq (f z) y).
-    + exfalso. eapply Hneq. eapply Hinj.
-      unfold extend. now rewrite Heq', Coqlib.peq_true.
+    + exfalso. eapply Hneq. eapply Hinj. now constructor.
+      now constructor. rewrite extend_gso; eauto.
+      rewrite extend_gss. eassumption.
     + edestruct (Henv z); eauto.
       constructor; eauto. intros Hc. inv Hc. congruence. 
       eexists. rewrite M.gso; eauto. 
@@ -410,7 +332,8 @@ Proof.
       simpl. rewrite Coqlib.peq_true. eauto.
     + edestruct IHHa as [xs2 [ e2 Ha' ] ]; eauto.
       edestruct (Coqlib.peq (f g) (f g0)). 
-      * eapply Hinj in e0. subst. congruence.
+      * eapply Hinj in e0. subst. congruence. now constructor.
+        now constructor.
       * do 2 eexists. simpl. rewrite Coqlib.peq_false; eauto.
 Qed.
 
@@ -464,8 +387,8 @@ Proof.
       * eexists. unfold extend. rewrite Coqlib.peq_false; [| now eauto ].
         rewrite M.gso; [ now eauto |].
         intros Heq. eapply n. 
-        eapply H7. unfold extend. rewrite Coqlib.peq_false; [| eassumption ].
-        rewrite Coqlib.peq_true. eassumption. 
+        eapply H7; try now constructor.
+        rewrite extend_gss. rewrite extend_gso; eassumption. 
 Qed.
  
 Lemma preord_env_P_inj_def_funs_pre k rho1 rho2 B1 B1' B2 B2' f h h' e :
@@ -525,6 +448,7 @@ Proof.
     rewrite Union_Empty_set_l. now apply Included_refl.
 Qed.
 
+(** α-equivalence preserves semantics *)
 Lemma Alpha_conv_correct k rho1 rho2 e1 e2 f :
   injective f ->
   Alpha_conv e1 e2 f ->
@@ -583,5 +507,5 @@ Proof.
       eauto. 
 Qed.
 
-Close Scope alpha_scope.
+Close Scope fun_scope.
 Close Scope ctx_scope.
